semantics/vyperEventScript.sml
@@ -1,0 +1,92 @@
+(*
+ * Concrete EVM event encoding for the Vyper semantics.
+ *
+ * TOP-LEVEL:
+ *   event_info       -- checked metadata needed to encode declared events
+ *   encode_vyper_event -- encode a declared Vyper event as an EVM event
+ *   encode_raw_event -- construct an EVM event for raw_log
+ *)
+
+Theory vyperEvent
+Ancestors
+  cv cv_std vyperABI vyperValue contractABI vfmTypes
+  byte keccak
+Libs
+  cv_transLib
+
+Type event_info = “:string -> (num # type list # bool list) option”
+
+Definition is_event_bytestring_type_def:
+  is_event_bytestring_type (BaseT (BytesT (Dynamic _))) = T ∧
+  is_event_bytestring_type (BaseT (StringT _)) = T ∧
+  is_event_bytestring_type _ = F
+End
+
+(* Primitive word encoding used for indexed, statically-sized arguments. *)
+Definition event_value_to_word_def:
+  event_value_to_word (BoolV b) = (if b then 1w else 0w : bytes32) ∧
+  event_value_to_word (IntV n) = (i2w n : bytes32) ∧
+  event_value_to_word (FlagV k) = (n2w k : bytes32) ∧
+  event_value_to_word (DecimalV n) = (i2w n : bytes32) ∧
+  event_value_to_word (BytesV bs) =
+    (if LENGTH bs = 20 then word_of_bytes_be (PAD_LEFT 0w 32 bs)
+     else word_of_bytes_be (PAD_RIGHT 0w 32 bs)) ∧
+  event_value_to_word _ = 0w
+End
+
+Definition encode_event_topic_def:
+  encode_event_topic T (BytesV bs) =
+    SOME (word_of_bytes_be (Keccak_256_w64 bs)) ∧
+  encode_event_topic T (StringV s) =
+    SOME (word_of_bytes_be (Keccak_256_w64 (MAP (n2w o ORD) s))) ∧
+  encode_event_topic T _ = NONE ∧
+  encode_event_topic F v = SOME (event_value_to_word v)
+End
+
+Definition encode_indexed_event_topics_def:
+  encode_indexed_event_topics [] [] [] = SOME ([] : bytes32 list) ∧
+  encode_indexed_event_topics (T::fs) (ty::tys) (v::vs) =
+    (case encode_event_topic (is_event_bytestring_type ty) v of
+     | NONE => NONE
+     | SOME topic =>
+         OPTION_MAP (CONS topic) (encode_indexed_event_topics fs tys vs)) ∧
+  encode_indexed_event_topics (F::fs) (_::tys) (_::vs) =
+    encode_indexed_event_topics fs tys vs ∧
+  encode_indexed_event_topics _ _ _ = NONE
+End
+
+Definition non_indexed_event_args_def:
+  non_indexed_event_args [] [] [] = SOME ([] : (type # value) list) ∧
+  non_indexed_event_args (T::fs) (_::tys) (_::vs) =
+    non_indexed_event_args fs tys vs ∧
+  non_indexed_event_args (F::fs) (ty::tys) (v::vs) =
+    OPTION_MAP (CONS (ty,v)) (non_indexed_event_args fs tys vs) ∧
+  non_indexed_event_args _ _ _ = NONE
+End
+
+Definition encode_vyper_event_def:
+  encode_vyper_event event_info tenv (logger : address) event_name vals =
+    case event_info event_name of
+    | NONE => NONE
+    | SOME (event_hash, arg_types, indexed_flags) =>
+        case encode_indexed_event_topics indexed_flags arg_types vals of
+        | NONE => NONE
+        | SOME indexed_topics =>
+            case non_indexed_event_args indexed_flags arg_types vals of
+            | NONE => NONE
+            | SOME typed_vals =>
+                case vyper_to_abi_list tenv (MAP FST typed_vals)
+                                            (MAP SND typed_vals) of
+                | NONE => NONE
+                | SOME abi_vals =>
+                    SOME <| logger := logger;
+                            topics := n2w event_hash :: indexed_topics;
+                            data := enc (Tuple (vyper_to_abi_types tenv
+                                                (MAP FST typed_vals)))
+                                        (ListV abi_vals) |>
+End
+
+Definition encode_raw_event_def:
+  encode_raw_event (logger : address) topics data : event =
+    <| logger := logger; topics := topics; data := data |>
+End
